coq/Util/ErrorSetoid.v
@@ -1,0 +1,139 @@
+Require Import Coq.Relations.Relations.
+Require Import Coq.Strings.String.
+
+Require Import MathClasses.interfaces.canonical_names.
+
+Require Export Vellvm.Error.
+
+Require Import Helix.Util.OptionSetoid.
+
+
+(* TODO: move to StringSetoid.v *)
+Section StringSetoid.
+
+  Global Instance string_Equiv : Equiv string :=
+    fun a b => is_true (eqb a b).
+
+  Global Instance string_Equivalence:
+    @Equivalence string (string_Equiv).
+  Proof.
+    split.
+    -
+      intros x.
+      apply eqb_refl.
+    -
+      intros x y E.
+      unfold string_Equiv, is_true in *.
+      rewrite <- E.
+      apply eqb_sym.
+    -
+      intros a b c Eab Ebc.
+      unfold string_Equiv, is_true in *.
+      apply eqb_eq in Eab.
+      apply eqb_eq in Ebc.
+      rewrite Eab, Ebc.
+      apply eqb_refl.
+  Qed.
+
+End StringSetoid.
+
+Inductive err_equiv_r {A:Type} `{Equiv A} : relation (err A) :=
+| err_r_inr : forall a b, a=b -> err_equiv_r (inr a) (inr b)
+| err_r_inl : forall a b, a=b -> err_equiv_r (inl a) (inl b).
+
+Global Instance err_equiv {T:Type} `{Equiv T}:
+  Equiv (err T) := err_equiv_r.
+
+
+Global Instance err_Equivalence
+       {A:Type}
+       `{Ae: Equiv A}
+       `{Ar: Equivalence A Ae}:
+  Equivalence (@err_equiv A Ae).
+Proof.
+  split.
+  -
+    intros x.
+    destruct x; constructor; try reflexivity.
+  -
+    intros x y E.
+    destruct x, y; inversion E; constructor; auto.
+  -
+    intros a b c Eab Ebc.
+    destruct a,b,c; inversion Eab; inversion Ebc;  constructor; auto.
+Qed.
+
+Global Instance err_inr_proper {T:Type} `{Equiv T}:
+  Proper ((=) ==> (=)) inr.
+Proof.
+  simpl_relation.
+  constructor.
+  assumption.
+Qed.
+
+Global Instance err_inl_proper {T:Type} `{Equiv T}:
+  Proper ((=) ==> (=)) inl.
+Proof.
+  simpl_relation.
+  constructor.
+  assumption.
+Qed.
+
+Global Instance trywith_proper {T:Type} `{Te: Equiv T}:
+  Proper((=) ==> (=) ==> (=)) (@trywith string T err Monad_err Exception_err).
+Proof.
+  simpl_relation.
+  unfold trywith.
+  destruct x0, y0; try some_none; try some_inv; try constructor; auto.
+Qed.
+
+Ltac destruct_err_equiv :=
+  match goal with
+  | [ |- @equiv (err _) (@err_equiv _ _) _ _] =>
+    unfold equiv; destruct_err_equiv
+  | [ |- err_equiv _ _] =>
+    unfold err_equiv; destruct_err_equiv
+  | [ |- err_equiv_r ?a ?b] =>
+    let Ha := fresh "Ha" in
+    let Hb := fresh "Hb" in
+    destruct a eqn:Ha, b eqn:Hb;
+    match goal with
+    | [ |- err_equiv_r (inr _) (inl _)] => exfalso
+    | [ |- err_equiv_r (inl _) (inr _)] => exfalso
+    | [ |- err_equiv_r (inl _) (inl _)] => constructor
+    | [ |- err_equiv_r (inr _) (inr _)] => constructor
+    end
+  end.
+
+(* Not 'err'-specific but defined here for lack of better place *)
+Ltac inl_inr :=
+  match goal with
+  | [H1: inl _ ≡ inr _ |- _] => inversion H1
+  | [H1: inr _ ≡ inl _ |- _] => inversion H1
+  | [H1: inl _ = inr _ |- _] => unfold equiv in H1; inversion H1
+  | [H1: inr _ = inl _ |- _] => unfold equiv in H1; inversion H1
+  | [ |- inl ?x ≡ inl ?x ] => reflexivity
+  | [ |- inr ?x ≡ inr ?x ] => reflexivity
+  | [H1: ?a = inr _,
+         H2: ?b = inl _ |- _] => rewrite H1 in H2;
+                               unfold equiv in H2;
+                               inversion H2
+  end.
+
+Lemma err_equiv_eq
+      {A: Type}
+      `{Ae: Equiv A}
+      `{Ar: Equivalence A Ae}
+      (a b: err A) :
+  (a ≡ b) -> (a = b).
+Proof.
+  intros H.
+  rewrite H.
+  reflexivity.
+Qed.
+
+Ltac err_eq_to_equiv_hyp :=
+  repeat
+    match goal with
+    | [H: @eq (err _) _ _ |- _] => apply err_equiv_eq in H
+    end.
